\section{Афанасьев. Задание 2}

\textbf{Постановка задачи:}
Взять неберущийся интеграл:
$$\int_{0}^{+ \infty}{ \frac{1}{ \sigma \sqrt{2 \pi}} e^{-
\frac{(x+M)^2}{2 \sigma^2}} dx}$$
с помощью табулированной функции:
$$Q(x)= \frac{1}{ \sqrt{2 \pi}} \int_{- \infty}^{x}{e^{-
\frac{z^2}{2}} dz}.$$

\textbf{Решение:}
$$
\int_{0}^{+ \infty}{ \frac{1}{ \sigma \sqrt{2 \pi}} e^{-
\frac{(x+M)^2}{2 \sigma^2}} dx}=
\frac{1}{ \sigma \sqrt{2 \pi}} \int_{0}^{+ \infty}{e^{-
\frac{1}{2} ( \frac{x+M}{ \sigma})^2} dx}=
\begin{vmatrix}
z= \frac{x+M}{ \sigma} \\
dz=z' dx= \frac{1}{ \sigma} dx \\
dx= \sigma dz \\
a= \frac{0+M}{ \sigma}= \frac{M}{ \sigma} \\
b= \frac{+ \infty +M}{ \sigma}=+ \infty
\end{vmatrix}=
$$
$$
=\frac{1}{ \sigma \sqrt{2 \pi}} \int_{ \frac{M}{ \sigma}}^{+ \infty}{e^{-
\frac{z^2}{2}} \sigma dz}=
\frac{1}{ \sqrt{2 \pi}} \int_{ \frac{M}{ \sigma}}^{+ \infty}{e^{-
\frac{z^2}{2}} dz}=
Q(+ \infty)-Q \bigg ( \frac{M}{ \sigma} \bigg )
$$